src/tls/test/TestClient13.fst
@@ -27,42 +27,10 @@ let config =
 	 ciphersuites = csn;
 	 }
 
-let id = {
-    msId = noMsId;
-    kdfAlg = PRF_SSL3_nested;
-    pv = TLS_1p3;
-    aeAlg = (AEAD CoreCrypto.AES_128_GCM CoreCrypto.SHA256);
-    csrConn = bytes_of_hex "";
-    ext = {
-      ne_extended_ms = false;
-      ne_extended_padding = false;
-      ne_secure_renegotiation = RI_Unsupported;
-      ne_supported_curves = None;
-      ne_supported_point_formats = None;
-      ne_server_names = None;
-      ne_signature_algorithms = None;
-      ne_keyShare = None
-    };
-    writer = Client
-  }
-
-let encryptor_TLS13_AES_GCM_128_SHA256 kv iv: writer id = 
-    // needed to match length requirements?
-    let kv: StreamAE.key id = kv |> unsafe_coerce in
-    let iv: StreamAE.iv id  = iv |> unsafe_coerce in
-
-    assume (~ (authId id));
-    StreamAE.coerce HyperHeap.root id kv iv
-
-let decryptor_TLS13_AES_GCM_128_SHA256 kv iv: reader id = 
-  let wr = encryptor_TLS13_AES_GCM_128_SHA256 kv iv in 
-  genReader HyperHeap.root wr
-
-
 //CF 16-04-30 it may be better to pass in a "Content.fragment i"
 
-val encryptRecord_TLS13_AES_GCM_128_SHA256: writer id -> Content.contentType -> bytes -> bytes
-let encryptRecord_TLS13_AES_GCM_128_SHA256 w ct plain = 
+val encryptRecord_TLS13_AES_GCM_128_SHA256: #id:id -> writer id -> Content.contentType -> bytes -> bytes
+let encryptRecord_TLS13_AES_GCM_128_SHA256 #id w ct plain = 
   // let pv = TLS_1p3 in
   let text = plain in
   // Range.frange -> Range.range
@@ -72,31 +40,13 @@ let encryptRecord_TLS13_AES_GCM_128_SHA256 w ct plain =
   let f = Content.mk_fragment id ct rg plain in 
   StreamAE.encrypt w (len+1) f // the extra byte is for CT with no padding
 
-(* was:
-  match ct with
-  |  Content.Application_data -> 
-       let f: DataStream.fragment id rg = text |> unsafe_coerce in
-       let f: StreamPlain.plain id (len+1) = Content.CT_Data #id rg f |> unsafe_coerce in
-         StreamAE.encrypt w (len+1) f
-  |  Content.Handshake ->
-       let f: StreamPlain.plain id (len+1) = Content.CT_Handshake #id rg text |> unsafe_coerce in
-         StreamAE.encrypt w (len+1) f
-*)
-
-
-let decryptRecord_TLS13_AES_GCM_128_SHA256 rd ct cipher = 
+val decryptRecord_TLS13_AES_GCM_128_SHA256: #id:id -> reader id -> Content.contentType -> bytes -> bytes
+let decryptRecord_TLS13_AES_GCM_128_SHA256 #id rd ct cipher = 
 //  IO.print_string ("cipher:"^(Platform.Bytes.print_bytes cipher)^"\n");
   let (Some d) = StreamAE.decrypt #id rd (length cipher - (StreamAE.ltag id)) cipher in
   Content.repr id d
 
-(* We should use Content.mk_fragment |> Content.repr, not Record.makePacket *)
-(* Even better, we should move to TLS.send *)
-//let makePacket ct ver (data: b:bytes { repr_bytes (length b) <= 2}) =
-//      abyte 22z
-//   @| versionBytes ver
-//   @| bytes_of_int 2 (length data) 
-//   @| data 
-
+// ADL 05/05: tried the top-level but still fails
 let sendRecord tcp pv ct msg str = 
   let r = Record.makePacket ct pv msg in
   let Correct _ = Platform.Tcp.send tcp r in
@@ -161,95 +111,54 @@ let recvEncAppDataRecord tcp pv rd =
   IO.print_string ((iutf8 payload)^"\n");
   payload
 
-(* Flex Handshake *)
-
-let deriveKeys_TLS13_AES_GCM_128_SHA256 (secret:bytes) (phase:string) (context:bytes) = 
-  let cekb = HSCrypto.hkdf_expand_label CoreCrypto.SHA256
-      	     secret (phase ^ ", client write key") context 16 in
-  let civb = HSCrypto.hkdf_expand_label CoreCrypto.SHA256
-      	     secret (phase ^ ", client write iv") context 12 in
-  let sekb = HSCrypto.hkdf_expand_label CoreCrypto.SHA256
-      	     secret (phase ^ ", server write key") context 16 in
-  let sivb = HSCrypto.hkdf_expand_label CoreCrypto.SHA256
-      	     secret (phase ^ ", server write iv") context 12 in
-  (cekb,civb,sekb,sivb)
-
-let derive_handshake_keys (gxy:CommonDH.secret) (log:bytes) = 
-  let log_hash = CoreCrypto.hash CoreCrypto.SHA256 log in
-  let zeroes = Platform.Bytes.abytes (String.make 32 (Char.char_of_int 0)) in
-  let xES = HSCrypto.hkdf_extract CoreCrypto.SHA256 zeroes gxy in
-  IO.print_string ("zeroes:"^(Platform.Bytes.print_bytes zeroes)^"\n");
-  IO.print_string ("gxy:"^(Platform.Bytes.print_bytes gxy)^"\n");
-  IO.print_string ("xES:"^(Platform.Bytes.print_bytes xES)^"\n");
-  let (ck,civ,sk,siv) = deriveKeys_TLS13_AES_GCM_128_SHA256 xES "handshake key expansion" log_hash in
-  IO.print_string ("client AES_GCM write log_hash:"^(Platform.Bytes.print_bytes log_hash)^"\n");
-  IO.print_string ("client AES_GCM write key:"^(Platform.Bytes.print_bytes ck)^"\n");
-  IO.print_string ("client AES_GCM salt: iv:"^(Platform.Bytes.print_bytes civ)^"\n");
-  IO.print_string ("server AES_GCM write key:"^(Platform.Bytes.print_bytes sk)^"\n");
-  IO.print_string ("server AES_GCM salt:"^(Platform.Bytes.print_bytes siv)^"\n");
-  (xES,ck,civ,sk,siv)
-
-let derive_finished_keys (xSS:bytes) (xES:bytes) (log:bytes) = 
-  let log_hash = CoreCrypto.hash CoreCrypto.SHA256 log in
-  let mSS = HSCrypto.hkdf_expand_label CoreCrypto.SHA256
-            xSS "expanded static secret" log_hash 32 in
-  let mES = HSCrypto.hkdf_expand_label CoreCrypto.SHA256
-            xES "expanded ephemeral secret" log_hash 32 in
-  let ms = HSCrypto.hkdf_extract CoreCrypto.SHA256 mSS mES in	    
-  let cfk = HSCrypto.hkdf_expand_label CoreCrypto.SHA256
-            ms "client finished" empty_bytes 32 in
-  let sfk = HSCrypto.hkdf_expand_label CoreCrypto.SHA256
-            ms "server finished" empty_bytes 32 in
-  let ts0 = HSCrypto.hkdf_expand_label CoreCrypto.SHA256
-            ms "traffic secret" log_hash 32 in
-  (ms,cfk,sfk,ts0)  
-  
-
+// Workaround until KeySchedule is merged in Handshake
+let replace_keyshare gn gx e =
+  match e with
+  | TLSExtensions.E_keyShare _ -> TLSExtensions.E_keyShare (ClientKeyShare [gn, CommonDH.serialize gx])
+  | x -> x 
 
 let main host port =
   IO.print_string "===============================================\n Starting test TLS client...\n";
   let tcp = Platform.Tcp.connect host port in
   let log = empty_bytes in
+  let rid = new_region root in
+  let ks = KeySchedule.create #rid config Client in
   
   let (Some gx,ch,chb) = Handshake.prepareClientHello config None None in
-  let pv = ch.ch_protocol_version in 
+  let cr, [(gn, gx)] = KeySchedule.ks_client_13_init_1rtt ks [SEC CoreCrypto.ECC_P256] in
+
+  let pv = ch.ch_protocol_version in
+  let hash x = CoreCrypto.hash CoreCrypto.SHA256 x in
   let kex = TLSConstants.Kex_ECDHE in
+  let ch = {ch with
+    ch_client_random = cr;
+    ch_extensions = (match ch.ch_extensions with
+      | None -> None
+      | Some l -> Some (List.Tot.map (replace_keyshare gn gx) l));} in
+
   let log = sendHSRecord tcp pv (ClientHello ch) log in
 
   let ServerHello(sh),log = recvHSRecord tcp pv kex log in
   let Correct (n,ake) = Handshake.processServerHello config None [] ch sh in
   let pv = sh.sh_protocol_version in
   let cs = sh.sh_cipher_suite in
-  let CipherSuite kex sa ae = cs in
 
   let Some (SEC ec,gyb) = n.n_extensions.ne_keyShare in
   let Correct gyb = vlparse 1 gyb in 
   IO.print_string ("server gy:"^(Platform.Bytes.print_bytes gyb)^"\n");
-
-  let Some gyp = ECGroup.parse_point gx.ec_params gyb in  
-  let gy = {ec_params = gx.ec_params; ec_point = gyp; ec_priv = None} in
-  let gxy = CommonDH.dh_initiator (CommonDH.ECKey gx) (CommonDH.ECKey gy) in
-  let (xES,ck,civ,sk,siv) = derive_handshake_keys gxy log in
-  let wr = encryptor_TLS13_AES_GCM_128_SHA256 ck civ in
-  let rd = decryptor_TLS13_AES_GCM_128_SHA256 sk siv in
-
-  let l = CoreCrypto.aeadRealIVSize (alg id) in
-  let extended = bytes_of_int l 0 in
-  let aeIV = xor l extended siv in
-  IO.print_string ("aeIV:"^(Platform.Bytes.print_bytes aeIV)^"\n");
+  let Some gy = CommonDH.parse (CommonDH.key_params gx) gyb in
+  let KeySchedule.StAEInstance rd wr = KeySchedule.ks_client_13_1rtt ks cs (gn, gy) (hash log) in
 
   let EncryptedExtensions(ee),log = recvEncHSRecord tcp pv kex log rd in
   let Certificate(sc),log = recvEncHSRecord tcp pv kex log rd in
   let CertificateVerify(cv),log = recvEncHSRecord tcp pv kex log rd in
-  let (ms,cfk,sfk,ts0) = derive_finished_keys xES xES log in
+//  let (ms,cfk,sfk,ts0) = derive_finished_keys xES xES log in
+  let svd = KeySchedule.ks_client_13_1rtt_server_finished ks (hash log) in
   let Finished(sfin),log = recvEncHSRecord tcp pv kex log rd in
+  // TODO check server finished
 
-  let log_hash = CoreCrypto.hash CoreCrypto.SHA256 log in
-  let (ck,civ,sk,siv) = deriveKeys_TLS13_AES_GCM_128_SHA256 ts0 "application data key expansion" log_hash in
-  let dwr = encryptor_TLS13_AES_GCM_128_SHA256 ck civ in
-  let drd = decryptor_TLS13_AES_GCM_128_SHA256 sk siv in
-  
-  let cfin = {fin_vd = CoreCrypto.hmac CoreCrypto.SHA256 cfk (CoreCrypto.hash CoreCrypto.SHA256 log)} in 
+  let cvd, (KeySchedule.StAEInstance drd dwr) = KeySchedule.ks_client_13_1rtt_client_finished ks (hash log) in
+  let cfin = {fin_vd = cvd} in
   let (str,cfinb,log) = makeHSRecord pv (Finished cfin) log in
   IO.print_string "before encrypt \n";
   let efinb = encryptRecord_TLS13_AES_GCM_128_SHA256 wr Content.Handshake cfinb in
@@ -259,36 +168,5 @@ let main host port =
   let get = encryptRecord_TLS13_AES_GCM_128_SHA256 dwr Content.Application_data (utf8 payload) in
   sendRecord tcp pv Content.Application_data get "GET /";
   let ad = recvEncAppDataRecord tcp pv drd in
-
-  
-
-(*  
-  let ms = TLSPRF.prf (pv,cs) pms (utf8 "master secret") (ch.ch_client_random @| sh.sh_server_random)  48 in
-  IO.print_string ("master secret:"^(Platform.Bytes.print_bytes ms)^"\n");
-  let (ck,civ,sk,siv) = deriveKeys_TLS12_AES_GCM_128_SHA256 ms ch.ch_client_random sh.sh_server_random in
-  IO.print_string ("client AES_GCM write key:"^(Platform.Bytes.print_bytes ck)^"\n");
-  IO.print_string ("client AES_GCM salt: iv:"^(Platform.Bytes.print_bytes civ)^"\n");
-  IO.print_string ("server AES_GCM write key:"^(Platform.Bytes.print_bytes sk)^"\n");
-  IO.print_string ("server AES_GCM salt:"^(Platform.Bytes.print_bytes siv)^"\n");
-
-  let cfin = {fin_vd = TLSPRF.verifyData (pv,cs) ms Client log} in 
-  let (str,cfinb,log) = makeHSRecord pv (Finished cfin) log in
-  let efinb = encryptRecord_TLS12_AES_GCM_128_SHA256 wr Content.Handshake cfinb in
-  sendRecord tcp pv Content.Change_cipher_spec HandshakeMessages.ccsBytes "Client";
-  sendRecord tcp pv Content.Handshake efinb str;
-
-  let _ = recvCCSRecord tcp pv in
-  let Finished(sfin),log = recvEncHSRecord tcp pv kex log rd in
-
-  let payload = "GET / HTTP/1.1\r\nHost: " ^ host ^ "\r\n\r\n" in
-  let get = encryptRecord_TLS12_AES_GCM_128_SHA256 wr Content.Application_data (utf8 payload) in
-
-  sendRecord tcp pv Content.Application_data get "GET /";
-  let ad = recvEncAppDataRecord tcp pv rd in
-*)
   ()
-
-  
-
-
 
